Convolution of k-regular sequences

Clemens Heuberger

Daniel Krenn

July 31, 2023

Remark 0.1. For matrices A and B, let $A \otimes B$ denote their tensor product. Then for matrices A, A_0 , A_1 , B, B_0 , B_1 of appropriate dimensions, we have

$$(A_0 \otimes B) + (A_1 \otimes B) = (A_0 + A_1) \otimes B$$
$$(A \otimes B_0) + (A \otimes B_1) = A \otimes (B_0 + B_1)$$

and

$$(A_0 \otimes B_0)(A_1 \otimes B_1) = (A_0 A_1) \otimes (B_0 B_1).$$

Note that for scalars a and b, we may identify $ab = (a) \otimes (b)$, where (a) and (b) are 1×1 -matrices.

For a linear representation (u_X, X, w_X) of a k-regular sequence x, we denote its right vector-valued sequence by $v_X(n) := \prod_{j=0}^{\ell-1} X(n_j) w_X$ if $n = (n_{\ell-1} \dots n_0)_k$ is the standard binary expansion of n. In particular, we have $x(n) = u_X^\top v_X(n)$ for all $n \ge 0$ and $v_X(0) = w_X$.

Theorem A. Let x and y be k-regular sequences with linear representations (u_X, X, w_X) and (u_Y, Y, w_Y) , respectively. Then the convolution

$$z = \left(\sum_{0 \le j \le n} x(j) y(n-j)\right)_{n \ge 0}$$

of x and y is k-regular with linear representation

$$\left(\begin{pmatrix} u_X \otimes u_Y \\ 0 \\ 0 \end{pmatrix}, Z, \begin{pmatrix} w_X \otimes w_Y \\ 0 \\ 0 \end{pmatrix} \right)$$

satisfying

$$Z(0) = \begin{pmatrix} A_0 & B_0 & 0 \\ 0 & A_{k-1} & B_{k-1} \\ 0 & A_{k-2} & B_{k-2} \end{pmatrix}, \quad Z(1) = \begin{pmatrix} A_1 & B_1 & 0 \\ A_0 & B_0 & 0 \\ 0 & A_{k-1} & B_{k-1} \end{pmatrix}$$

and

$$Z(r) = \begin{pmatrix} A_r & B_r & 0 \\ A_{r-1} & B_{r-1} & 0 \\ A_{r-2} & B_{r-2} & 0 \end{pmatrix} \quad \text{for all } r \ge 2,$$

with

$$A_r = \sum_{0 \le s \le r} (X(s) \otimes Y(r-s)), \quad B_r = \sum_{r < s < k} (X(s) \otimes Y(k+r-s))$$

for all $0 \le r < k$.

Lemma 0.2. Suppose we are in the set-up of Theorem A. Let v_X and v_Y be the right vector-valued sequences associated with the linear representations (u_X, X, w_X) and (u_Y, Y, w_Y) , respectively, and define

$$v'(n) := \sum_{0 \le j \le n} v_X(j) \otimes v_Y(n-j).$$

Then

$$z = \left((u_X^\top \otimes u_Y^\top) v'(n) \right)_{n \ge 0}.$$

Proof. We have

$$z(n) = \sum_{0 \le j \le n} u_X^\top v_X(j) u_Y^\top v_Y(n-j) = (u_X^\top \otimes u_Y^\top) \sum_{0 \le j \le n} (v_X(j) \otimes v_Y(n-j))$$
$$= (u_X^\top \otimes u_Y^\top) v'(n)$$

which proves the lemma.

Lemma 0.3. Suppose we are in the set-up of Theorem A. The right vector-valued sequence v' of Lemma 0.2 satisfies

$$v'(kn + r) = A_r v'(n) + B_r v'(n - 1)$$

for all $n \ge 0$ and $0 \le r < k$ with

$$A_r = \sum_{0 \le s \le r} (X(s) \otimes Y(r-s)), \quad B_r = \sum_{r < s < k} (X(s) \otimes Y(k+r-s))$$

for all $0 \le r < k$ and where v'(-1) = 0 because it is an empty sum.

Proof. For $n \ge 0$ and $0 \le r < k$, we obtain

$$\begin{split} v'(kn+r) &= \sum_{0 \leq j \leq kn+r} v_X(j) \otimes v_Y(kn+r-j) \\ &= \sum_{0 \leq ki+s \leq kn+r} v_X(ki+s) \otimes v_Y(k(n-i)+r-s) \\ &= \sum_{0 \leq s \leq r} v_X(ki+s) \otimes v_Y(k(n-i)+r-s) \\ &+ \sum_{\substack{r < s < k \\ 0 \leq i \leq n-1}} v_X(ki+s) \otimes v_Y(k(n-i-1)+k+r-s) \\ &= \sum_{\substack{0 \leq s \leq r \\ 0 \leq i \leq n}} (X(s)v_X(i)) \otimes (Y(r-s)v_Y(n-i)) \\ &+ \sum_{\substack{r < s < k \\ 0 \leq i \leq n}} (X(s)v_X(i)) \otimes (Y(k+r-s)v_Y(n-i-1)) \\ &= \sum_{\substack{0 \leq s \leq r \\ 0 \leq i \leq n-1}} (X(s) \otimes Y(r-s)) \sum_{\substack{0 \leq i \leq n-1}} (v_X(i) \otimes v_Y(n-i-1)) \\ &+ \sum_{r < s < k} (X(s) \otimes Y(k+r-s)) \sum_{\substack{0 \leq i \leq n-1}} (v_X(i) \otimes v_Y(n-i-1)) \\ &= \sum_{0 \leq s \leq r} (X(s) \otimes Y(r-s))v'(n) + \sum_{r < s < k} (X(s) \otimes Y(k+r-s))v'(n-1). \end{split}$$

Proposition 0.4. Let $z = (u'v'(n))_{n\geq 0}$ be a k-regular sequence with left vector u' and right vector-valued sequence v' satisfying

$$v'(kn + r) = A_r v'(n) + B_r v'(n - 1)$$

for all $n \ge 0$ and $0 \le r < k$ with some matrices A_r and B_r for all $0 \le r < k$. Then z has a linear representation

$$\left(\begin{pmatrix} u' \\ 0 \\ 0 \end{pmatrix}, Z, \begin{pmatrix} v'(0) \\ 0 \\ 0 \end{pmatrix} \right)$$

with right vector-valued sequence $v_Z(n) = (v'(n), v'(n-1), v'(n-2))^{\top}$ and satisfying

$$Z(0) = \begin{pmatrix} A_0 & B_0 & 0 \\ 0 & A_{k-1} & B_{k-1} \\ 0 & A_{k-2} & B_{k-2} \end{pmatrix}, \quad Z(1) = \begin{pmatrix} A_1 & B_1 & 0 \\ A_0 & B_0 & 0 \\ 0 & A_{k-1} & B_{k-1} \end{pmatrix}$$

and

$$Z(r) = \begin{pmatrix} A_r & B_r & 0 \\ A_{r-1} & B_{r-1} & 0 \\ A_{r-2} & B_{r-2} & 0 \end{pmatrix} \quad \text{for all } r \ge 2.$$

Proof. The result is a straight-forward generalization (from scalar coefficients)	ents to our
matrix-valued coefficients A_r and B_r) of a special case of [2, Theorem A]. It	can also be
easily verified by a direct computation.	
Proof of Theorem A. The convolution z of the two k -regular sequences x and again k -regular; see [1, Theorem 3.1]. The linear representation follows by Lemma 0.2, Lemma 0.3 and Proposition 0.4.	0

References

- [1] Jean-Paul Allouche and Jeffrey Shallit, The ring of k-regular sequences, Theoret. Comput. Sci. **98** (1992), no. 2, 163–197. MR 1166363
- [2] Clemens Heuberger, Daniel Krenn, and Gabriel F. Lipnik, Asymptotic analysis of q-recursive sequences, Algorithmica 84 (2022), no. 9, 2480–2532. MR 4467813